importing binnat for testing

theories/test_CoqEAL.v
@@ -2,83 +2,11 @@ From mathcomp Require Import ssreflect ssrfun ssrbool eqtype ssrnat div seq.
 From mathcomp Require Import path choice fintype tuple finset bigop.
 
 From elpi Require Import elpi.
-Require Import test_param.
+Require Import test_param hrel ops.
 
 Set Implicit Arguments.
 Unset Strict Implicit.
 Unset Printing Implicit Defensive.
-
-Delimit Scope rel_scope with rel.
-
-(***************************)
-(* Heterogeneous Relations *)
-(***************************)
-Section hrel.
-
-Definition sub_hrel A B (R R' : A -> B -> Type) :=
-  forall (x : A) (y : B), R x y -> R' x y.
-
-Notation "X <= Y" := (sub_hrel X%rel Y%rel) : rel_scope.
-
-Inductive eq_hrel A B (R R' : A -> B -> Type) :=
-  EqHrel of (R <= R')%rel & (R' <= R)%rel.
-
-Notation "X <=> Y" := (eq_hrel X Y) (format "X  <=>  Y", at level 95) : rel_scope.
-
-Lemma eq_hrelRL A B (R R' : A -> B -> Type) : (R <=> R')%rel -> (R <= R')%rel.
-Proof. by case. Qed.
-
-Lemma eq_hrelLR A B (R R' : A -> B -> Type) : (R <=> R')%rel -> (R' <= R)%rel.
-Proof. by case. Qed.
-
-Definition comp_hrel A B C
-  (R : A -> B -> Type) (R' : B -> C -> Type) : A -> C -> Type :=
-    fun a c => sigT (fun b => R a b * R' b c)%type.
-
-Notation "X \o Y" := (comp_hrel X Y) : rel_scope.
-
-Lemma comp_hrelP A B C (R : A -> B -> Type) (R' : B -> C -> Type)
-  (b : B) (a : A) (c : C) : R a b -> R' b c -> (R \o R')%rel a c.
-Proof. by exists b. Qed.
-
-Definition prod_hrel A A' B B' (rA : A -> A' -> Type) (rB : B -> B' -> Type) :
-  A * B -> A' * B' -> Type :=
-  fun x y => (rA x.1 y.1 * rB x.2 y.2)%type.
-
-Lemma comp_eqr A B (R : A -> B -> Type) : (R \o eq <= R)%rel.
-Proof. by move=> x y [y' [? <-]]. Qed.
-
-Lemma comp_eql A B (R : A -> B -> Type) : (eq \o R <= R)%rel.
-Proof. by move=> x y [y' [<-]]. Qed.
-
-Definition fun_hrel A B (f : B -> A) : A -> B -> Type :=
-  fun a b => f b = a.
-
-Definition ofun_hrel A B (f : B -> option A) : A -> B -> Type :=
-  fun a b => f b = Some a.
-
-Definition hrespectful (A B C D : Type)
-  (R : A -> B -> Type) (R' : C -> D -> Type) : (A -> C) -> (B -> D) -> Type :=
-  fun f g => forall (x : A) (y : B), R x y -> R' (f x) (g y).
-
-Notation " R ==> S " := (@hrespectful _ _ _ _ R%rel S%rel)
-    (right associativity, at level 55) : rel_scope.
-
-Lemma sub_hresp_comp A B C (R1 R1' : A -> B -> Prop) (R2 R2' : B -> C -> Prop) :
-  (((R1 ==> R1') \o (R2 ==> R2')) <= ((R1 \o R2) ==> (R1' \o R2')))%rel.
-Proof.
-move=> f h [g [rfg rgh]] x z [y [rxy ryz]]; exists (g y).
-by split; [apply: rfg | apply: rgh].
-Qed.
-
-End hrel.
-
-Notation "X \o Y" := (comp_hrel X%rel Y%rel) : rel_scope.
-Notation "X <= Y" := (sub_hrel X%rel Y%rel) : rel_scope.
-Notation "X <=> Y" := (eq_hrel X%rel Y%rel) (format "X  <=>  Y", at level 95) : rel_scope.
-Notation " R ==> S " := (@hrespectful _ _ _ _ R%rel S%rel)
-    (right associativity, at level 55) : rel_scope.
-
 
 Class refines X Y (R : X -> Y -> Type) x y : Type := Refines : R x y.
 Arguments refines {_ _} R%rel _ _.
@@ -89,9 +17,7 @@ Lemma refines_apply
   forall (a : A) (b : B), refines R a b ->
   forall (c : A -> C) (d : B -> D), refines (R ==> R') c d ->
    refines R' (c a) (d b).
-Proof.
-
-Admitted.
+Proof. by move=> a b Rab c d; apply. Qed.
 
 Cd "~/git/coq-elpi".
 Elpi Run param "with-TC-param (param {{O}} X Y)".
@@ -100,6 +26,360 @@ Elpi Tactic coqeal " typecheck. ".
 Elpi Accumulate File "coq-extra.elpi".
 Elpi Accumulate File "coq-EAL.elpi".
 Elpi Run coqeal " typecheck ".
+
+Require Import ZArith pos.
+
+Section positive_op.
+
+Definition positive_of_pos (p : pos) : positive := Pos.of_nat (val p).
+Definition pos_of_positive (p : positive) : pos := insubd pos1 (Pos.to_nat p).
+
+Global Instance spec_positive   : Op.spec_of positive pos := pos_of_positive.
+Global Instance implem_positive : Op.implem_of pos positive := positive_of_pos.
+Global Instance one_positive    : Op.one_of positive := xH.
+Global Instance add_positive    : Op.add_of positive := Pos.add.
+Global Instance sub_positive    : Op.sub_of positive := Pos.sub.
+Global Instance mul_positive    : Op.mul_of positive := Pos.mul.
+Global Instance le_positive     : Op.leq_of positive := Pos.leb.
+Global Instance lt_positive     : Op.lt_of positive  := Pos.ltb.
+Global Instance eq_positive     : Op.eq_of positive  := Pos.eqb.
+Global Instance exp_positive    : Op.exp_of positive positive := Pos.pow.
+End positive_op.
+
+Section positive_theory.
+
+Local Open Scope rel_scope.
+
+Lemma positive_of_posK : cancel positive_of_pos pos_of_positive.
+Proof.
+move=> n /=; rewrite /positive_of_pos /pos_of_positive /=.
+apply: val_inj; rewrite Nat2Pos.id ?insubdK -?topredE ?valP //.
+by apply/eqP; rewrite -lt0n valP.
+Qed.
+
+Lemma to_natE : forall (p : positive), Pos.to_nat p = nat_of_pos p.
+Proof.
+by elim=> //= p <-;
+rewrite ?Pos2Nat.inj_xI ?Pos2Nat.inj_xO NatTrec.trecE -mul2n.
+Qed.
+
+Lemma to_nat_gt0 p : 0 < Pos.to_nat p.
+Proof.
+by rewrite to_natE; elim: p => //= p; rewrite NatTrec.trecE double_gt0.
+Qed.
+Hint Resolve to_nat_gt0.
+
+Lemma pos_of_positiveK : cancel pos_of_positive positive_of_pos.
+Proof.
+move=> n /=; rewrite /positive_of_pos /pos_of_positive /=.
+by rewrite val_insubd to_nat_gt0 Pos2Nat.id.
+Qed.
+
+Definition Rpos := fun_hrel pos_of_positive.
+
+Lemma RposE (p : pos) (x : positive) :
+  refines Rpos p x -> p = pos_of_positive x.
+Proof. by []. Qed.
+
+Lemma RposI (p : pos) (x : positive) :
+  refines Rpos p x -> x = positive_of_pos p.
+Proof. by move=> /RposE ->; rewrite pos_of_positiveK. Qed.
+
+Global Instance Rpos_spec_pos_r x : refines Rpos (Op.spec x) x.
+Proof. by []. Qed.
+
+(* Global Instance Rpos_spec_pos_l : refines (Rpos ==> pos_R) spec_id spec. *)
+(* Proof. *)
+(*   rewrite refinesE=> x x'. *)
+(*   rewrite -[Rpos]refinesE=> rx. *)
+(*   rewrite [spec _]RposE [y in pos_of_positive y]RposI positive_of_posK /spec_id. *)
+(*   exact: pos_Rxx. *)
+(* Qed. *)
+
+Global Instance Rpos_spec : refines (Rpos ==> Logic.eq) Op.spec_id Op.spec.
+Proof. by rewrite []. Qed.
+
+Global Instance Rpos_implem : refines (Logic.eq ==> Rpos) Op.implem_id implem.
+Proof.
+  rewrite refinesE=> _ x ->.
+  case: x=> n ngt0.
+  by rewrite /Rpos /fun_hrel positive_of_posK.
+Qed.
+
+Global Instance Rpos_1 : refines Rpos (pos1 : pos) (1%C : positive).
+Proof. by rewrite !refinesE; apply: val_inj; rewrite /= insubdK. Qed.
+
+Global Instance Rpos_add : refines (Rpos ==> Rpos ==> Rpos) add_pos +%C.
+Proof.
+rewrite refinesE => _ x <- _ y <-; apply: val_inj.
+rewrite !val_insubd Pos2Nat.inj_add.
+by move: (Pos2Nat.is_pos x) (Pos2Nat.is_pos y) => /leP -> /leP ->.
+Qed.
+
+Global Instance Rpos_mul : refines (Rpos ==> Rpos ==> Rpos) mul_pos *%C.
+Proof.
+rewrite refinesE => _ x <- _ y <-; apply: val_inj.
+rewrite !val_insubd Pos2Nat.inj_mul.
+by move: (Pos2Nat.is_pos x) (Pos2Nat.is_pos y) => /leP -> /leP ->.
+Qed.
+
+Global Instance Rpos_sub : refines (Rpos ==> Rpos ==> Rpos) sub_pos sub_op.
+Proof.
+rewrite refinesE => _ x <- _ y <-; apply: val_inj; rewrite !val_insubd.
+move: (Pos2Nat.is_pos x) (Pos2Nat.is_pos y) => /leP -> /leP ->.
+have [/leP h|/leP h] := (ltnP (Pos.to_nat y) (Pos.to_nat x)).
+  by have := (Pos2Nat.inj_sub x y); rewrite Pos2Nat.inj_lt => ->.
+rewrite /sub_op /sub_positive Pos.sub_le ?Pos2Nat.inj_le //.
+by rewrite subn_gt0 !ltnNge; move/leP: h ->.
+Qed.
+
+Global Instance Rpos_leq : refines (Rpos ==> Rpos ==> bool_R) leq_pos Op.leq.
+Proof.
+  rewrite refinesE=> _ x <- _ y <-;
+  rewrite /leq_op /le_positive /leq_pos !val_insubd.
+  move: (Pos2Nat.is_pos x) (Pos2Nat.is_pos y) => /leP -> /leP ->.
+  by case: (Pos.leb_spec0 _ _); move /Pos2Nat.inj_le /leP;
+  [move ->|rewrite -eqbF_neg; move/eqP ->].
+Qed.
+
+Global Instance Rpos_lt : refines (Rpos ==> Rpos ==> bool_R) lt_pos Op.lt.
+Proof.
+rewrite refinesE => /= _ x <- _ y <-; rewrite /lt_pos !val_insubd.
+move: (Pos2Nat.is_pos x) (Pos2Nat.is_pos y) => /leP -> /leP ->.
+have -> : (Pos.to_nat x < Pos.to_nat y) = (x < y)%C.
+  by apply/ltP/idP => [|h]; rewrite -Pos2Nat.inj_lt -Pos.ltb_lt.
+exact: bool_Rxx.
+Qed.
+
+Global Instance Rpos_eq : refines (Rpos ==> Rpos ==> bool_R) eq_pos Op.eq.
+Proof.
+  rewrite refinesE=> _ x <- _ y <-; rewrite /eq_op /eq_positive /eq_pos.
+  case: (Pos.eqb_spec _ _)=> [->|h].
+    by rewrite eqxx.
+  suff H : (pos_of_positive x == pos_of_positive y) = false.
+    by rewrite H.
+  by apply/negP=> [/eqP /(can_inj pos_of_positiveK)].
+Qed.
+
+Lemma pos2nat_inj_exp x y : Pos.to_nat (x ^ y) = Pos.to_nat x ^ Pos.to_nat y.
+Proof.
+  have pos2nat_pow_xO a b
+       (hab : Pos.to_nat (a ^ b) = Pos.to_nat a ^ Pos.to_nat b) :
+    Pos.to_nat (a ^ b~0) = (Pos.to_nat a ^ Pos.to_nat b) ^ 2.
+    by rewrite -Z2Nat.inj_pos Pos2Z.inj_pow Pos2Z.inj_xO Z.mul_comm Z.pow_mul_r
+               // Z.pow_2_r -Pos2Z.inj_pow Z2Nat.inj_mul // Z2Nat.inj_pos multE
+               hab mulnn.
+  elim: y=> [y ihy|y ihy|].
+      by rewrite Pos2Nat.inj_xI multE expnS [in _ ^ _]mulnC expnM Pos.xI_succ_xO
+                 Pos.pow_succ_r Pos2Nat.inj_mul multE pos2nat_pow_xO.
+    by rewrite Pos2Nat.inj_xO multE mulnC expnM pos2nat_pow_xO.
+  by rewrite Pos2Nat.inj_1 expn1 Pos.pow_1_r.
+Qed.
+
+Global Instance Rpos_exp : refines (Rpos ==> Rpos ==> Rpos) exp_pos exp_op.
+Proof.
+  rewrite refinesE /exp_op /exp_positive=> _ x <- _ y <-.
+  apply: val_inj.
+  by rewrite !val_insubd expn_gt0 !to_nat_gt0 pos2nat_inj_exp.
+Qed.
+
+End positive_theory.
+
+Typeclasses Opaque pos_of_positive positive_of_pos.
+Global Opaque pos_of_positive positive_of_pos.
+
+Section binnat_op.
+
+Global Instance zero_N : Op.zero_of N := N.zero.
+Global Instance one_N  : Op.one_of N  := N.one.
+Global Instance add_N  : Op.add_of N  := N.add.
+
+Definition succN (n : N) : N := (1 + n)%C.
+
+Global Instance sub_N  : Op.sub_of N := N.sub.
+Global Instance exp_N  : Op.exp_of N N := N.pow.
+Global Instance mul_N  : Op.mul_of N := N.mul.
+Global Instance div_N  : Op.div_of N := N.div.
+Global Instance mod_N  : Op.mod_of N := N.modulo.
+Global Instance eq_N   : Op.eq_of N  := N.eqb.
+Global Instance leq_N  : Op.leq_of N := N.leb.
+Global Instance lt_N   : Op.lt_of N  := N.ltb.
+
+Global Instance cast_positive_N : Op.cast_of positive N := Npos.
+Global Instance cast_N_positive : Op.cast_of N positive :=
+  fun n => if n is Npos p then p else 1%C.
+
+Global Instance spec_N : Op.spec_of N nat := nat_of_bin.
+Global Instance implem_N : Op.implem_of nat N := bin_of_nat.
+
+End binnat_op.
+
+Section binnat_theory.
+
+Local Open Scope rel_scope.
+
+Definition Rnat : nat -> N -> Type := fun_hrel nat_of_bin.
+Instance ref_Rnat : 'refinement Rnat.
+
+Lemma RnatE (n : nat) (x : N) : refines_rec Rnat n x -> n = x.
+Proof. by rewrite refinesE. Qed.
+
+Global Instance Rnat_spec_r x : refines Rnat (spec x) x.
+Proof. by rewrite refinesE. Qed.
+
+Global Instance Rnat_spec : refines (Rnat ==> Logic.eq) Op.spec_id spec.
+Proof. by rewrite refinesE. Qed.
+
+Global Instance Rnat_implem : refines (Logic.eq ==> Rnat) Op.implem_id implem.
+Proof.
+rewrite !refinesE => x _ <-.
+by rewrite /Rnat /fun_hrel /implem /implem_N bin_of_natK.
+Qed.
+
+Global Instance Rnat_0 : refines Rnat 0 0%C.
+Proof. by rewrite refinesE. Qed.
+
+Global Instance Rnat_1 : refines Rnat 1%nat 1%C.
+Proof. by rewrite refinesE. Qed.
+
+Global Instance Rnat_add : refines (Rnat ==> Rnat ==> Rnat) addn +%C.
+Proof.
+by rewrite refinesE => _ x <- _ y <-; rewrite /Rnat /fun_hrel nat_of_add_bin.
+Qed.
+
+(* Hint Extern 999 (@refinement _ _ _) => *)
+(*   (once lazymatch goal with |- ?g => idtac "trying " g; fail 1 end) *)
+(*  : typeclass_instances. *)
+
+
+Global Instance Rnat_S : refines (Rnat ==> Rnat) S succN.
+Proof. by refines_abstrE; rewrite -add1n; apply/spec_refines. Qed.
+
+Lemma nat_of_binK : forall x, N.of_nat (nat_of_bin x) = x.
+Proof.
+by case => //= p; apply: Nnat.N2Nat.inj; rewrite Nnat.Nat2N.id /= to_natE.
+Qed.
+
+Global Instance Rnat_sub : refines (Rnat ==> Rnat ==> Rnat) subn sub_op.
+Proof.
+rewrite refinesE => _ x <- _ y <-.
+by apply: Nnat.Nat2N.inj; rewrite Nnat.Nat2N.inj_sub !nat_of_binK.
+Qed.
+
+Global Instance Rnat_mul : refines (Rnat ==> Rnat ==> Rnat) muln mul_op.
+Proof.
+rewrite refinesE => _ x <- _ y <-.
+by rewrite /Rnat /fun_hrel /= nat_of_mul_bin.
+Qed.
+
+Global Instance Rnat_div_eucl :
+  refines (Rnat ==> Rnat ==> prod_R Rnat Rnat) edivn N.div_eucl.
+Proof.
+rewrite refinesE /Rnat /fun_hrel=> _ x <- _ y <-.
+rewrite edivn_def /=.
+case: x=> [|x] /=; first by rewrite div0n mod0n.
+case: y=> [|y] //=.
+have hspec := N.pos_div_eucl_spec x (N.pos y).
+have hrem := N.pos_div_eucl_remainder x (N.pos y).
+destruct N.pos_div_eucl.
+rewrite -[nat_of_pos _]/(nat_of_bin (N.pos _)) hspec /= {hspec}.
+rewrite nat_of_add_bin nat_of_mul_bin.
+have rem_lt_div : (n0 < N.pos y)%N.
+  have pos_ne0 : N.pos y <> 0%num by [].
+  have /= := hrem pos_ne0.
+  rewrite /N.lt Nnat.N2Nat.inj_compare /= to_natE.
+  move/nat_compare_lt/ltP.
+  case: n0 {hrem}=> //= p.
+  by rewrite to_natE.
+rewrite modnMDl modn_small ?rem_lt_div // divnMDl /= -?to_natE ?to_nat_gt0 //.
+by rewrite divn_small ?addn0 // ?to_natE.
+Qed.
+
+Global Instance Rnat_div : refines (Rnat ==> Rnat ==> Rnat) divn div_op.
+Proof.  refines_abstrE; rewrite /divn; apply/spec_refines. Qed.
+
+Global Instance Rnat_mod : refines (Rnat ==> Rnat ==> Rnat) modn mod_op.
+Proof. by refines_abstrE; rewrite modn_def; apply/spec_refines. Qed.
+
+Global Instance Rnat_exp : refines (Rnat ==> Rnat ==> Rnat) expn exp_op.
+Proof.
+  rewrite refinesE => _ x <- _ y <-; rewrite /Rnat /fun_hrel /=.
+  rewrite /exp_op /exp_N /N.pow.
+  case: x y => [|x] [|y] //.
+    rewrite exp0n //=; elim: y => //= p.
+    by rewrite natTrecE double_gt0.
+  have nat_of_binposE p : nat_of_bin (N.pos p) = Pos.to_nat p.
+    elim: p=> [p ihp|p ihp|] /=; last (by rewrite Pos2Nat.inj_1);
+      by rewrite ?(Pos2Nat.inj_xI, Pos2Nat.inj_xO) multE NatTrec.doubleE to_natE
+                 mul2n.
+  by rewrite !nat_of_binposE pos2nat_inj_exp.
+Qed.
+
+Global Instance Rnat_eq : refines (Rnat ==> Rnat ==> bool_R) eqtype.eq_op Op.eq.
+Proof.
+rewrite refinesE=> _ x <- _ y <-; rewrite /eq_op /eq_N.
+case: (N.eqb_spec _ _) => [->|/eqP hneq]; first by rewrite eqxx.
+suff H : (nat_of_bin x == nat_of_bin y) = false by rewrite H.
+by apply/negP => [/eqP /(can_inj nat_of_binK)]; apply/eqP.
+Qed.
+
+Global Instance refines_spec_bool : 
+  refines (bool_R ==> eq) Op.spec_id id.
+Proof. by rewrite refinesE => ??[]. Qed.
+
+Global Instance Rnat_leq : refines (Rnat ==> Rnat ==> bool_R) ssrnat.leq Op.leq.
+Proof.
+rewrite refinesE=> _ x <- _ y <-; rewrite /leq_op /leq_N /leq.
+case: (N.leb_spec0 _ _)=> [/N.sub_0_le|] xBy.
+  by rewrite [_ == _](coqeal unify) [sub_op _ _]xBy.
+suff H : (nat_of_bin x - nat_of_bin y == 0) = false.
+  by rewrite /(_ <= _)%N H.
+apply/negP=> /eqP; rewrite [x - y]RnatE [0]RnatE.
+by move/(can_inj nat_of_binK)/N.sub_0_le.
+Qed.
+
+Global Instance Rnat_lt : refines (Rnat ==> Rnat ==> bool_R) ltn lt_op.
+Proof.
+refines_abstr; rewrite refinesE /ltn /= ltnNge; apply/eq_spec_refines.
+by rewrite /lt_op /lt_N N.ltb_antisym.
+Qed.
+
+Global Instance Rnat_cast_positive_N :
+  refines (Rpos ==> Rnat) val (cast : positive -> N).
+Proof.
+  rewrite refinesE /cast /Rnat /fun_hrel => x x' rx.
+  by rewrite [x]RposE val_insubd to_nat_gt0 to_natE.
+Qed.
+
+Global Instance Rnat_cast_N_positive :
+  refines (Rnat ==> Rpos) (insubd pos1) (cast : N -> positive).
+Proof.
+  rewrite refinesE=> x x' rx; rewrite [x]RnatE.
+  case: x' {x rx} => [|p] /=; last by rewrite -to_natE.
+  rewrite /insubd insubF //= /cast.
+  by apply (@spec_refinesP _ _ _ _ _ _ _ _ _).
+Qed.
+
+End binnat_theory.
+
+Typeclasses Opaque nat_of_bin bin_of_nat.
+Global Opaque nat_of_bin bin_of_nat.
+
+Section test.
+
+Instance : 'refinement Rnat.
+
+Lemma test : 10000%num * 10000%num * (99999999%num + 1) =
+             10000000000000000%num.
+Proof.
+by rewrite [X in X = _](coqeal unify); reflexivity.
+Qed.
+
+Lemma test' : 10000%num * 10000%num * (99999999%num + 1) =
+             10000000000000000%num.
+Proof. by apply/eqP; rewrite [_ == _](coqeal unify). Qed.
+
+End test.
 
 
 Section CoqEAL.
@@ -115,10 +395,6 @@ Context {Rone : refines R 1 one}.
 Context {Radd : refines (R ==> R ==> R)%rel addn add}.
 
 Context {Rfrombool : forall b, refines R (nat_of_bool b) (N_of_bool b)}.
-(* Elpi Tactic coqeal "easy {{addn}} {{@Radd}}.". *)
-
-(* Elpi Run coqeal "coq-locate ""refines"" (const GR), *)
-(*                  coq-TC-db-for GR L.". *)
 
 Lemma test_refines0 : { x : _ & refines R 1 x}.
 Proof.
@@ -149,6 +425,7 @@ Lemma test_refines_big : { x : N & refines R (0 + ((0 + (((((0 + ((0 + ((0 + 1))
 Proof.
   eexists.
   Time elpi coqeal; shelve_unifiable.
+Show Proof.
 Qed.
 
 Elpi Run coqeal "
